src/Narcissus/BinLib/AlignedMonads.v
@@ -10,10 +10,10 @@ Require Import
         Fiat.Narcissus.BinLib.AlignedByteString.
 
 Section AlignedDecodeM.
-  
+
   Context {cache : Cache}.
   Context {cacheAddNat : CacheAdd cache nat}.
-    
+
   Definition AlignedDecodeM
              (A : Set)
              (n : nat):=
@@ -21,22 +21,84 @@ Section AlignedDecodeM.
     -> nat
     -> CacheDecode
     -> option (A * nat * CacheDecode).
-  
+
   Definition BindAlignedDecodeM
              {A B : Set}
              {n : nat}
              (a : AlignedDecodeM A n)
              (b : A -> AlignedDecodeM B n)
     : AlignedDecodeM B n :=
-    fun v idx c => (Ifopt a v n c  as a' Then (b (fst (fst a')) v (snd (fst a')) (snd a')) Else None).
-  
+    fun v idx c => (Ifopt a v idx c  as a' Then (b (fst (fst a')) v (snd (fst a')) (snd a')) Else None).
+
   Definition ReturnAlignedDecodeM
              {A : Set}
              {n : nat}
              (a : A)
     : AlignedDecodeM A n :=
-    fun v idx c => Some (a, n, c).
- 
+    fun v idx c => Some (a, idx, c).
+
+  Definition AlignedDecodeMEquiv
+             {A} {n}
+             (a1 a2 : AlignedDecodeM A n) : Prop :=
+    forall v idx c, a1 v idx c = a2 v idx c.
+
+  Lemma AlignedDecodeMEquiv_refl {A : Set} {n}:
+    forall (a : AlignedDecodeM A n),
+      AlignedDecodeMEquiv a a.
+  Proof.
+    unfold AlignedDecodeMEquiv; intros; reflexivity.
+  Qed.
+
+  Lemma AlignedDecodeMEquiv_sym {A : Set} {n}:
+    forall (a1 a2 : AlignedDecodeM A n),
+      AlignedDecodeMEquiv a1 a2 -> AlignedDecodeMEquiv a2 a1.
+  Proof.
+    unfold AlignedDecodeMEquiv; intros; congruence.
+  Qed.
+
+  Lemma AlignedDecodeMEquiv_trans {A : Set} {n}:
+    forall (a1 a2 a3 : AlignedDecodeM A n),
+      AlignedDecodeMEquiv a1 a2 ->
+      AlignedDecodeMEquiv a2 a3 ->
+      AlignedDecodeMEquiv a1 a3.
+  Proof.
+    unfold AlignedDecodeMEquiv; intros; congruence.
+  Qed.
+
+  Global Instance PreOrder_AlignedDecodeMEquiv {A : Set} {n} :
+    PreOrder (@AlignedDecodeMEquiv A n) :=
+    {| PreOrder_Reflexive := AlignedDecodeMEquiv_refl;
+       PreOrder_Transitive := AlignedDecodeMEquiv_trans|}.
+
+  Lemma BindAlignedDecodeM_assoc {A B C : Set} {n}:
+    forall (a : AlignedDecodeM A n)
+           (f : A -> AlignedDecodeM B n)
+           (g : B -> AlignedDecodeM C n),
+      AlignedDecodeMEquiv (BindAlignedDecodeM (BindAlignedDecodeM a f) g)
+                          (BindAlignedDecodeM a (fun a => BindAlignedDecodeM (f a) g)).
+  Proof.
+    unfold BindAlignedDecodeM, AlignedDecodeMEquiv; simpl; intros.
+    destruct (a v idx c); simpl; eauto.
+  Qed.
+
+  Lemma ReturnAlignedDecodeM_LeftUnit {A B : Set} {n}:
+    forall (a : A)
+           (f : A -> AlignedDecodeM B n),
+      AlignedDecodeMEquiv (BindAlignedDecodeM (ReturnAlignedDecodeM a) f)
+                          (f a).
+  Proof.
+    unfold ReturnAlignedDecodeM, BindAlignedDecodeM, AlignedDecodeMEquiv; simpl; intros.
+    reflexivity.
+  Qed.
+
+  Lemma ReturnAlignedDecodeM_RightUnit {A B : Set} {n}:
+    forall (f : AlignedDecodeM A n),
+      AlignedDecodeMEquiv (BindAlignedDecodeM f ReturnAlignedDecodeM) f.
+  Proof.
+    unfold ReturnAlignedDecodeM, BindAlignedDecodeM, AlignedDecodeMEquiv; simpl; intros.
+    destruct (f v idx c) as [ [ [? ?] ?] | ] ; simpl; reflexivity.
+  Qed.
+
   Definition ThrowAlignedDecodeM
              {A : Set}
              {n : nat}
@@ -49,19 +111,121 @@ Section AlignedDecodeM.
     (v : Vector.t A n)
     (m : nat)
     : option A :=
-    match n, v with
+    match m, v with
     | 0,  Vector.cons a _ _ => Some a
     | S m', Vector.cons _ _ v' => nth_opt v' m'
     | _, _ => None
     end.
-  
+
   Definition GetCurrentByte (* Gets the current byte and increments the current index. *)
-             {A : Set}
              {n : nat}
-             (m : AlignedDecodeM A n)
     : AlignedDecodeM char n :=
-    fun v idx c => Ifopt (nth_opt v idx) as b Then Some (b, S idx, c) Else None.
-  
-End AlignedDecodeM. 
+    fun v idx c => Ifopt (nth_opt v idx) as b Then Some (b, S idx, addD c 8) Else None.
 
+  (* Equivalence Criteria:
+     A bit-aligned decoder and byte-aligned decoder are equivalent when
+     - the byte aligned decoder fails when the bit aligned decoder does,
+     - decodes the same values as the bit-aligned decoder
+     - updates the cache in the same way as the bit-aligned decoder,
+       - and consumes the same number of bytes as the bit-aligned decoder.
+   *)
 
+  Definition DecodeMEquivAlignedDecodeM
+             {C : Set}
+             (f : DecodeM C ByteString)
+             (f' : forall {numBytes}, AlignedDecodeM C numBytes)
+    := (forall {numBytes_hd}
+               (n : nat)
+               (v : Vector.t _ (S numBytes_hd)) cd,
+           f' v (S n) cd =
+           Ifopt (f' (Vector.tl v) n cd) as a Then Some (fst (fst a), S (snd (fst a)), snd a) Else None)
+       /\ (forall b cd c b' cd', f b cd = Some (c, b', cd')
+                                 -> length_ByteString b >= length_ByteString b')%nat
+       /\ (forall n (v : Vector.t (word 8) n) cd,
+              (f (build_aligned_ByteString v) cd = None <->
+               f' v 0 cd = None)
+              /\
+              (forall c bs' cd',
+                  f (build_aligned_ByteString v) cd = Some (c, bs', cd') ->
+                  f' v 0 cd = Some (c, n - (numBytes bs'), cd')))
+       /\ (forall n m o (v : Vector.t (word 8) (n + (m + o))) cd c cd' H,
+              f' v n cd = Some (c, o, cd') ->
+              f (build_aligned_ByteString (snd (Vector_split n (m + o) v))) cd =
+              Some (c, build_aligned_ByteString (snd (Vector_split (n + m) o (eq_rect _ _ v _ H))), cd')
+          ).
+
+  Lemma DecodeMEquivAlignedDecodeM_trans  {C} :
+    forall bit_decoder1 byte_decoder1 bit_decoder2 byte_decoder2,
+      DecodeMEquivAlignedDecodeM (C := C) bit_decoder1 byte_decoder1
+      -> (forall b cd, bit_decoder1 b cd  = bit_decoder2 b cd)
+      -> (forall n, AlignedDecodeMEquiv (byte_decoder1 n) (byte_decoder2 n))
+      -> DecodeMEquivAlignedDecodeM bit_decoder2 byte_decoder2.
+  Proof.
+    unfold DecodeMEquivAlignedDecodeM; intros; intuition; rewrite <- ?H0, <- ?H1; eauto.
+    - eapply H; rewrite H0; eauto.
+    - eapply H3; rewrite H0; eauto.
+    - eapply H3; rewrite H1; eauto.
+    - eapply H3; rewrite H0; eauto.
+    - eapply H5; rewrite H1; eauto.
+  Qed.
+
+  Lemma Return_DecodeMEquivAlignedDecodeM {A : Set}
+        (a : A)
+    : DecodeMEquivAlignedDecodeM
+        (fun (b : ByteString) (cd : CacheDecode) => Some (a, b, cd))
+     (fun numBytes => ReturnAlignedDecodeM a).
+  Proof.
+    unfold DecodeMEquivAlignedDecodeM; intros; intuition.
+    - injections; eauto.
+    - discriminate.
+    - discriminate.
+    - unfold ReturnAlignedDecodeM, numBytes; injections.
+      simpl; repeat f_equal; omega.
+    - unfold ReturnAlignedDecodeM in H0; injections; simpl.
+      repeat f_equal.
+  Admitted.
+
+  Lemma Bind_DecodeMEquivAlignedDecodeM {A C : Set}
+        (A_decode : DecodeM A ByteString)
+        (A_decode_aligned : forall {numBytes}, AlignedDecodeM A numBytes)
+        (t : A -> DecodeM C ByteString)
+        (t' : A -> forall {numBytes}, AlignedDecodeM C numBytes)
+    : DecodeMEquivAlignedDecodeM A_decode (@A_decode_aligned)
+      -> (forall a, DecodeMEquivAlignedDecodeM (t a) (@t' a))
+      -> DecodeMEquivAlignedDecodeM
+     (fun (b : ByteString) (c : CacheDecode) =>
+        `(a, bs, cd') <- A_decode b c; t a bs cd')
+     (fun numBytes => BindAlignedDecodeM A_decode_aligned (fun a => @t' a numBytes)).
+  Proof.
+    unfold DecodeMEquivAlignedDecodeM; intros; intuition.
+    - unfold BindAlignedDecodeM.
+      rewrite H1.
+      destruct (A_decode_aligned numBytes_hd (Vector.tl v) n cd) as [ [ [? ?] ?] | ]; simpl.
+      + specialize (H0 a); intuition.
+      + reflexivity.
+    - eapply DecodeBindOpt2_inv in H3; destruct_ex; intuition.
+      specialize (H0 x); intuition.
+      eapply H in H5.
+      symmetry in H6; eapply H0 in H6; omega.
+    - destruct (A_decode (build_aligned_ByteString v) cd) as [ [ [? ?] ?] | ] eqn: ?;
+        simpl in *; try discriminate.
+      unfold BindAlignedDecodeM.
+      apply H2 in Heqo; destruct_ex; intuition; subst.
+      rewrite Heqo; simpl; eauto.
+      admit.
+      unfold BindAlignedDecodeM; eapply H2 in Heqo; rewrite Heqo; reflexivity.
+    - admit.
+    - eapply DecodeBindOpt2_inv in H3; destruct_ex; intuition.
+      eapply H2 in H5.
+      unfold BindAlignedDecodeM; rewrite H5; simpl.
+      symmetry in H6.
+      specialize (H0 x); intuition.
+      admit.
+    - admit.
+  Qed.
+
+End AlignedDecodeM.
+
+Delimit Scope AlignedDecodeM_scope with AlignedDecodeM.
+Notation "x <- y ; z" := (BindAlignedDecodeM y (fun x => z)) : AlignedDecodeM_scope.
+Notation "'return' x" := (ReturnAlignedDecodeM x) (at level 10): AlignedDecodeM_scope.
